Get rid of overlapping notations for Par.
Par is now defined as an expression of type [∀ X, expr X] (instead of a
value) and we prove that it is stable under weakening and substitution.

heap_lang/lib/par.v
@@ -2,17 +2,19 @@ From iris.heap_lang Require Export spawn.
 From iris.heap_lang Require Import proofmode notation.
 Import uPred.
 
-Definition par : val :=
+Definition par {X} : expr X :=
   λ: "fs",
     let: "handle" := ^spawn (Fst '"fs") in
     let: "v2" := Snd '"fs" #() in
     let: "v1" := ^join '"handle" in
     Pair '"v1" '"v2".
-Notation Par e1 e2 := (^par (Pair (λ: <>, e1) (λ: <>, e2)))%E.
-Notation ParV e1 e2 := (par (Pair (λ: <>, e1) (λ: <>, e2)))%E.
-(* We want both par and par^ to print like this. *)
-Infix "||" := ParV : expr_scope.
+Notation Par e1 e2 := (par (Pair (λ: <>, e1) (λ: <>, e2)))%E.
 Infix "||" := Par : expr_scope.
+
+Instance do_wexpr_assert {X Y} (H : X `included` Y) : WExpr H par par := _.
+Instance do_wsubst_assert {X Y} x es (H : X `included` x :: Y) :
+  WSubst x es H par par := do_wsubst_closed _ x es H _.
+Typeclasses Opaque par.
 
 Section proof.
 Context {Σ : gFunctors} `{!heapG Σ, !spawnG Σ}.
@@ -25,19 +27,19 @@ Lemma par_spec (Ψ1 Ψ2 : val → iProp) e (f1 f2 : val) (Φ : val → iProp) :
    ∀ v1 v2, Ψ1 v1 ★ Ψ2 v2 -★ ▷ Φ (v1,v2)%V)
   ⊢ WP par e {{ Φ }}.
 Proof.
-  iIntros {??} "(#Hh&Hf1&Hf2&HΦ)". wp_value. wp_let. wp_proj.
+  iIntros {??} "(#Hh&Hf1&Hf2&HΦ)". rewrite /par. wp_value. wp_let. wp_proj.
   wp_apply spawn_spec; try wp_done. iFrame "Hf1 Hh".
   iIntros {l} "Hl". wp_let. wp_proj. wp_focus (f2 _).
   iApply wp_wand_l; iFrame "Hf2"; iIntros {v} "H2". wp_let.
   wp_apply join_spec; iFrame "Hl". iIntros {w} "H1".
-  iSpecialize "HΦ" "-"; first by iSplitL "H1". wp_let. by iPvsIntro.
+  iSpecialize "HΦ" "-"; first by iSplitL "H1". by wp_let.
 Qed.
 
 Lemma wp_par (Ψ1 Ψ2 : val → iProp) (e1 e2 : expr []) (Φ : val → iProp) :
   heapN ⊥ N →
   (heap_ctx heapN ★ WP e1 {{ Ψ1 }} ★ WP e2 {{ Ψ2 }} ★
    ∀ v1 v2, Ψ1 v1 ★ Ψ2 v2 -★ ▷ Φ (v1,v2)%V)
-  ⊢ WP ParV e1 e2 {{ Φ }}.
+  ⊢ WP e1 || e2 {{ Φ }}.
 Proof.
   iIntros {?} "(#Hh&H1&H2&H)". iApply par_spec; auto.
   iFrame "Hh H". iSplitL "H1"; by wp_let.
