heap_lang/lib/assert.v
@@ -4,12 +4,12 @@ From iris.heap_lang Require Import wp_tactics substitution notation.
 Definition Assert {X} (e : expr X) : expr X :=
   if: e then #() else #0 #0. (* #0 #0 is unsafe *)
 
-Instance do_wsubst_assert {X Y} x es (H : X `included` x :: Y) e er :
-  WSubst x es H e er → WSubst x es H (Assert e) (Assert er) | 1.
-Proof. intros; red. by rewrite /Assert /wsubst -/wsubst; f_equal/=. Qed.
 Instance do_wexpr_assert {X Y} (H : X `included` Y) e er :
-  WExpr H e er → WExpr H (Assert e) (Assert er) | 1.
-Proof. intros; red. by rewrite /Assert /wexpr -/wexpr; f_equal/=. Qed.
+  WExpr H e er → WExpr H (Assert e) (Assert er) := _.
+Instance do_wsubst_assert {X Y} x es (H : X `included` x :: Y) e er :
+  WSubst x es H e er → WSubst x es H (Assert e) (Assert er).
+Proof. intros; red. by rewrite /Assert /wsubst -/wsubst; f_equal/=. Qed.
+Typeclasses Opaque Assert.
 
 Lemma wp_assert {Σ} (Φ : val → iProp heap_lang Σ) :
   ▷ Φ #() ⊢ WP Assert #true {{ Φ }}.
